Instances/Setoid/Mon.v
@@ -20,32 +20,150 @@ Coercion sgr : Mon >-> Sgr.
 
 Hint Resolve neutr_l neutr_r.
 
-Ltac mon_simpl := intros;
-match goal with
-  (* Neutral element of the operation. Not sure if works. *)
-  | H : context [?op neutr _] |- _ => rewrite neutr_l in H
-  | H : context [?op _ neutr] |- _ => rewrite neutr_r in H
-  | |- context [?op neutr _] => rewrite neutr_l
-  | |- context [?op _ neutr] => rewrite neutr_r
-  | f : ?X -> ?Y, X_neutr : ?X, pres_neutr : ?f ?X_neutr == ?neutr2 |- _ =>
-    match goal with
-      (* This can't be here because H gets rewritten in itself and thus
-         effectively destroyed. *)
-      (*| H : context [f ?neutr1] |- _ => rewrite pres_neutr in H*)
-      | |- context [?f ?neutr1] => rewrite pres_neutr
-    end
-  (* Homomorphisms *)
-  | f : ?X -> ?Y, H : ?f neutr == neutr |- context [?f neutr] =>
-    rewrite H
-  | _ => idtac
-end; sgr_simpl.
+Definition MonHom (X Y : Mon) : Type :=
+    {f : SgrHom X Y | f neutr == neutr}.
 
-Ltac mon_simpl2 := intros;
-match goal with
-  | X_neutr : ?X |- _ => match goal with
-    | op : X -> ?Y |- _ => clear
-  end
+Definition MonHom_SgrHom (X Y : Mon) (f : MonHom X Y)
+    : SgrHom X Y := proj1_sig f.
+Coercion MonHom_SgrHom : MonHom >-> SgrHom.
+
+Inductive exp (X : Mon) : Type :=
+    | Id : exp X
+    | Var : X -> exp X
+    | Op : exp X -> exp X -> exp X
+    | Mor : forall A : Mon, MonHom A X -> exp A -> exp X.
+
+Arguments Id [X].
+Arguments Var [X] _.
+Arguments Op [X] _ _.
+Arguments Mor [X A] _ _ .
+
+Fixpoint expDenote {X : Mon} (e : exp X) : X :=
+match e with
+    | Id => neutr
+    | Var v => v
+    | Op e1 e2 => op (expDenote e1) (expDenote e2)
+    | Mor f e' => f (expDenote e')
 end.
+
+Require Import List.
+Import ListNotations.
+
+Fixpoint simplify {X : Mon} (e : exp X) : exp X :=
+match e with
+    | Id => Id
+    | Var v => Var v
+    | Op e1 e2 =>
+        match simplify e1, simplify e2 with
+            | Id, e2' => e2'
+            | e1', Id => e1'
+            | e1', e2' => Op e1' e2'
+        end
+    | Mor f e' => match simplify e' with
+        | Id => Id
+        | Op e1 e2 => Op (Mor f e1) (Mor f e2)
+        | e'' => Mor f e''
+    end
+end.
+
+Theorem simplify_correct :
+  forall (X : Mon) (e : exp X),
+    expDenote (simplify e) == expDenote e.
+Proof.
+  induction e; simpl; pose (@op_Proper X).
+    reflexivity.
+    reflexivity.
+    destruct (simplify e1), (simplify e2); simpl in *; try
+    rewrite <- IHe1, <- IHe2; try rewrite neutr_l; try rewrite neutr_r;
+    try reflexivity.
+    destruct (simplify e); simpl in *; pose (wut := SgrHom_Proper m);
+    rewrite <- IHe.
+      destruct m; simpl in *. symmetry. assumption.
+      reflexivity.
+      destruct m, x; simpl in *. rewrite e1. reflexivity.
+      reflexivity.
+Qed.
+
+Fixpoint expDenoteL {X : Mon} (l : list X) : X :=
+match l with
+    | [] => neutr
+    | h :: t => op h (expDenoteL t)
+end.
+
+Lemma expDenoteL_app :
+  forall (X : Mon) (l1 l2 : list X),
+    expDenoteL (l1 ++ l2) == op (expDenoteL l1) (expDenoteL l2).
+Proof.
+  induction l1 as [| h1 t1]; simpl; intros.
+    rewrite neutr_l. reflexivity.
+    rewrite <- assoc. apply op_Proper.
+      reflexivity.
+      rewrite IHt1. reflexivity.
+Qed.
+
+Lemma expDenoteL_hom :
+  forall (X Y : Mon) (f : MonHom X Y) (l : list X),
+    expDenoteL (map f l) == f (expDenoteL l).
+Proof.
+  induction l as [| h t]; simpl.
+    destruct f; simpl in *. symmetry. assumption.
+    destruct f, x; simpl in *. rewrite e0. apply op_Proper.
+      reflexivity.
+      assumption.
+Qed.
+
+Fixpoint flatten {X : Mon} (e : exp X) : list X :=
+match e with
+    | Id => []
+    | Var v => [v]
+    | Op e1 e2 => flatten e1 ++ flatten e2
+    | Mor f e' => map f (flatten e')
+end.
+
+Theorem flatten_correct :
+  forall (X : Mon) (e : exp X),
+    expDenoteL (flatten e) == expDenote e.
+Proof.
+  induction e; simpl.
+    reflexivity.
+    rewrite neutr_r. reflexivity.
+    rewrite expDenoteL_app. apply op_Proper; assumption.
+    rewrite expDenoteL_hom. apply (SgrHom_Proper m); assumption.
+Qed.
+
+Theorem mon_reflect :
+  forall (X : Mon) (e1 e2 : exp X),
+    expDenoteL (flatten (simplify e1)) ==
+    expDenoteL (flatten (simplify e2)) ->
+      expDenote e1 == expDenote e2.
+Proof.
+  intros.
+  do 2 rewrite flatten_correct in H.
+  do 2 rewrite simplify_correct in H.
+  assumption.
+Qed.
+
+Ltac reify e :=
+lazymatch e with
+    | @neutr ?X => constr:(@Id X)
+    | op ?e1 ?e2 =>
+        let e1' := reify e1 in
+        let e2' := reify e2 in constr:(Op e1' e2')
+    | SetoidHom_Fun (SgrHom_Fun (MonHom_SgrHom ?f)) ?e =>
+        let e' := reify e in constr:(Mor f e')
+    | ?v => constr:(Var v)
+end.
+
+Ltac reflect_mon := simpl; intros;
+match goal with
+    | |- ?e1 == ?e2 =>
+        let e1' := reify e1 in
+        let e2' := reify e2 in
+          change (expDenote e1' == expDenote e2');
+          apply mon_reflect; simpl
+end.
+
+Ltac mon_simpl := sgr_simpl.
 
 Ltac monob M := try intros until M;
 match type of M with
@@ -68,13 +186,6 @@ end.
 Ltac monobs := monobs_template monob.
 Ltac monobs' := monobs_template monob'.
 
-Definition MonHom (X Y : Mon) : Type :=
-    {f : SgrHom X Y | f neutr == neutr}.
-
-Definition MonHom_SgrHom (X Y : Mon) (f : MonHom X Y)
-    : SgrHom X Y := proj1_sig f.
-Coercion MonHom_SgrHom : MonHom >-> SgrHom.
-
 Ltac monhom f := try intros until f;
 match type of f with
     | MonHom _ _ =>
@@ -93,153 +204,38 @@ end; mon_simpl.
 Ltac monhoms := monhoms_template monhom.
 Ltac monhoms' := monhoms_template monhom'.
 
-Ltac mon_aux :=
+Ltac mon := intros; try (reflect_mon; try reflexivity; fail); repeat
 match goal with
-  | |- (_, _) = _ => f_equal
-  | _ => cat
+    | |- _ == _ => reflect_mon; reflexivity
+    | |- Equivalence _ => solve_equiv
+    | |- Proper _ _ => proper
+    | |- (_, _) = (_, _) => f_equal
+    | _ => mon_simpl || monobs' || monhoms' || cat
 end.
-
-Ltac mon_wut := repeat (mon_simpl || monobs || monhoms || mon_aux || cat).
-Ltac mon := try (mon_wut; fail).
-
-Ltac mon_wut' := repeat (mon_simpl || monobs' || monhoms' || mon_aux || cat).
-Ltac mon' := try (mon_wut'; fail).
-
-Inductive exp : Mon -> Type :=
-    | Id : forall X : Mon, exp X
-    | Var : forall X : Mon, X -> exp X
-    | Op : forall X : Mon, exp X -> exp X -> exp X
-    | Mor : forall X Y : Mon, MonHom X Y -> exp X -> exp Y.
-
-Arguments Id [X].
-Arguments Var [X] _.
-Arguments Op [X] _ _.
-Arguments Mor [X Y] _ _ .
-
-Fixpoint expDenote {X : Mon} (e : exp X) : X :=
-match e with
-    | Id => neutr
-    | Var v => v
-    | Op e1 e2 => op (expDenote e1) (expDenote e2)
-    | Mor f e' => f (expDenote e')
-end.
-
-Require Import List.
-Import ListNotations.
-
-Fixpoint expDenoteL {X : Mon} (l : list X) : X :=
-match l with
-    | [] => neutr
-    | h :: t => op h (expDenoteL t)
-end.
-
-Fixpoint flatten {X : Mon} (e : exp X) : list X :=
-match e with
-    | Id => []
-    | Var v => [v]
-    | Op e1 e2 => flatten e1 ++ flatten e2
-    | Mor f Id => []
-    | Mor f e' => map f (flatten e')
-end.
-
-Lemma flatten_Hom : forall (X : Mon) (f : MonHom X X) (e : exp X),
-  e <> Id -> flatten (Mor f e) = map f (flatten e).
-Proof.
-  destruct e; auto.
-Qed.
-
-Lemma expDenoteL_app :
-  forall (X : Mon) (l1 l2 : list X),
-    expDenoteL (l1 ++ l2) == op (expDenoteL l1) (expDenoteL l2).
-Proof.
-  induction l1 as [| h1 t1]; simpl; intros.
-    rewrite neutr_l. reflexivity.
-    rewrite <- assoc. apply op_Proper.
-      reflexivity.
-      rewrite IHt1. reflexivity.
-Qed.
-
-Lemma expDenoteL_hom :
-  forall (X Y : Mon) (f : MonHom X Y) (l : list X),
-    expDenoteL (map f l) == f (expDenoteL l).
-Proof.
-  induction l as [| h t]; simpl.
-    mon'.
-    assert (f (op h (expDenoteL t)) == op (f h) (f (expDenoteL t))).
-      mon'.
-      rewrite H. apply op_Proper.
-        reflexivity.
-        assumption.
-Qed.
-
-Theorem flatten_correct :
-  forall (X : Mon) (e : exp X),
-    expDenoteL (flatten e) == expDenote e.
-Proof.
-  induction e.
-    reflexivity.
-    mon.
-    simpl. rewrite expDenoteL_app. apply op_Proper; assumption.
-    destruct e; simpl.
-      mon'.
-      mon'.
-      rewrite expDenoteL_hom. monhom' m. mon'.
-      rewrite expDenoteL_hom. mon'.
-Qed.
-
-Theorem mon_reflect :
-  forall (X : Mon) (e1 e2 : exp X),
-    expDenoteL (flatten e1) == expDenoteL (flatten e2) ->
-      expDenote e1 == expDenote e2.
-Proof.
-  induction e1; intros; repeat rewrite flatten_correct in H;
-  assumption.
-Qed.
-
-Ltac reify e :=
-lazymatch e with
-    | @neutr ?X => constr:(@Id X)
-    | op ?e1 ?e2 =>
-        let e1' := reify e1 in
-        let e2' := reify e2 in constr:(Op e1' e2')
-    | SetoidHom_Fun (SgrHom_Fun (MonHom_SgrHom ?f)) ?e =>
-        let e' := reify e in constr:(Mor f e')
-    | ?v => constr:(Var v)
-end.
-
-Ltac mon2 := simpl; intros;
-match goal with
-    | |- ?e1 == ?e2 =>
-        let e1' := reify e1 in
-        let e2' := reify e2 in
-          change (expDenote e1' == expDenote e2');
-          apply mon_reflect; simpl
-end.
-
-Ltac mon2' := mon2; try reflexivity.
 
 Goal forall (X : Mon) (a b c : X),
   op a (op b c) == op (op a b) c.
 Proof.
-  mon2'.
+  reflect_mon. reflexivity.
 Qed.
 
 Goal forall (X : Mon) (f : MonHom X X) (a b : X),
   f (op a b) == op (f a) (f b).
 Proof.
-  mon2'.
+  reflect_mon. reflexivity.
 Qed.
 
 Goal forall (X : Mon) (f : MonHom X X) (a b c : X),
   op (f (f neutr)) (op (f a) (f (op b c))) ==
   op (f a) (op (f b) (f c)).
 Proof.
-  mon2'.
+  reflect_mon. reflexivity.
 Qed.
 
 Goal forall (X Y Z : Mon) (f : MonHom X Y) (g : MonHom Y Z),
   g (f neutr) == neutr.
-Proof. mon2'.
+Proof.
+  reflect_mon. reflexivity.
 Qed.
 
 Instance MonHomSetoid (X Y : Mon) : Setoid (MonHom X Y) :=
@@ -252,11 +248,13 @@ Proof. apply Setoid_kernel_equiv. Defined.
 Definition MonComp (X Y Z : Mon) (f : MonHom X Y) (g : MonHom Y Z)
     : MonHom X Z.
 Proof.
-  red. exists (SgrComp f g). Time mon2'.
+  red. exists (SgrComp f g). mon.
 Defined.
 
 Definition MonId (X : Mon) : MonHom X X.
-Proof. red. exists (SgrId X). Time mon2'. Defined.
+Proof.
+  red. exists (SgrId X). mon.
+Defined.
 
 Instance MonCat : Cat :=
 {
@@ -266,10 +264,7 @@ Instance MonCat : Cat :=
     comp := MonComp;
     id := MonId
 }.
-Proof.
-  (* Proper *) proper. mon'.
-  (* Category laws *) Time all: mon'.
-Defined.
+Proof. all: mon. Defined.
 
 Instance Mon_init : Mon :=
 {
@@ -278,18 +273,19 @@ Instance Mon_init : Mon :=
 }.
 Proof. all: mon. Defined.
 
+Definition Mon_Setoid_create (X : Mon) : SetoidHom Mon_init X.
+Proof.
+  red. exists (fun _ => neutr). mon.
+Defined.
+
 Definition Mon_Sgr_create (X : Mon) : SgrHom Mon_init X.
 Proof.
-  Definition Mon_Setoid_create (X : Mon) : SetoidHom Mon_init X.
-  Proof.
-    red. exists (fun _ => neutr). proper.
-  Defined.
-  red. exists (Mon_Setoid_create X). Time mon2'.
+  red. exists (Mon_Setoid_create X). mon.
 Defined.
 
 Definition Mon_create (X : Mon) : Hom Mon_init X.
 Proof.
-  mon_simpl. exists (Mon_Sgr_create X). mon2'.
+  do 3 red. exists (Mon_Sgr_create X). mon.
 Defined.
 
 Instance Mon_has_init : has_init MonCat :=
@@ -306,18 +302,19 @@ Instance Mon_term : Mon :=
 }.
 Proof. all: mon. Defined.
 
+Definition Mon_Setoid_delete (X : Mon) : SetoidHom X Mon_term.
+Proof.
+  red. exists (fun _ => tt). mon.
+Defined.
+
 Definition Mon_Sgr_delete (X : Mon) : SgrHom X Mon_term.
 Proof.
-  Definition Mon_Setoid_delete (X : Mon) : SetoidHom X Mon_term.
-  Proof.
-    red. exists (fun _ => tt). proper.
-  Defined.
   red. exists (Mon_Setoid_delete X). mon.
 Defined.
 
 Definition Mon_delete (X : Mon) : Hom X Mon_term.
 Proof.
-  mon_simpl. exists (Mon_Sgr_delete X). mon.
+  do 3 red. exists (Mon_Sgr_delete X). mon.
 Defined.
 
 Instance Mon_has_term : has_term MonCat :=
@@ -354,7 +351,7 @@ Defined.
 Definition Mon_fpair (A B X : Mon) (f : MonHom X A) (g : MonHom X B)
     : MonHom X (Mon_prodOb A B).
 Proof.
-  red. exists (Sgr_fpair f g). mon.
+  red. exists (Sgr_fpair f g). (* TODO : make faster *) Time mon.
 Defined.
 
 Instance Mon_has_products : has_products MonCat :=
@@ -366,5 +363,5 @@ Instance Mon_has_products : has_products MonCat :=
 }.
 Proof.
   proper.
-  repeat red. intros. mon.
+  repeat split; cat. (* TODO : mon doesn't work *)
 Defined.
